\chapter{Elementary Algebra}

\M
The axioms for elementary algebra include the following statements,
which possibly include redundancies. We summarize results which may be
found, e.g., in Appendix C of Mayer~\cite{mayer:calculus}. Also note
that the accepted notation has:
\begin{subequations}
\begin{align}
  a - b &:= a + (-b)
  \intertext{and}
  a/b &:= a\cdot(b^{-1}).
\end{align}
\end{subequations}

\N{Commutativity laws}
\begin{enumerate}
\item $\forall a,b\in\RR, a+b=b+a$
\item $\forall a,b\in\RR, a\cdot b=b\cdot a$
\end{enumerate}

\N{Associativity laws}
\begin{enumerate}[resume*]
\item $\forall a,b,c\in\RR, (a+b)+c=a+(b+c)$
\item $\forall a,b,c\in\RR, (a\cdot b)\cdot c=a\cdot(b\cdot c)$
\end{enumerate}

\N{Left Distributive property}
\begin{enumerate}[resume*]
\item $\forall a,b,c\in\RR, a\cdot(b+c)=(a\cdot b)+(a\cdot c)$
\item $\forall a,b,c\in\RR, a\cdot(b-c)=(a\cdot b)-(a\cdot c)$
\end{enumerate}

\N{Right Distributive property}
\begin{enumerate}[resume*]
\item $\forall a,b,c\in\RR, (a+b)\cdot c=(a\cdot c)+(b\cdot c)$
\item $\forall a,b,c\in\RR, (a-b)\cdot c=(a\cdot c)-(b\cdot c)$
\item $\forall a,b,c\in\RR, (a+b)/c=(a/c)+(b/c)$
\item  $\forall a,b,c\in\RR, (a-b)/c=(a/c)-(b/c)$
\end{enumerate}

\N{Axioms of $0$ and $1$} The rational numbers $0$ and $1$ satisfies the
following axioms.

\begin{enumerate}[resume*]
\item $\forall a\in\RR, a+0=a$
\item $\forall a\in\RR, 0+a=a$
\item $\forall a\in\RR, a\cdot1=a$
\item $\forall a\in\RR, 1\cdot a=a$
\item $\forall a\in\RR, a\cdot0=0$
\item $\forall a\in\RR, 0\cdot a=0$
\item $0\neq1$
\item $\forall a,b\in\RR$, if $ab=0$, then $a=0$ or $b=0$ (or both)
\end{enumerate}

\N{Additive and multiplicative Inverse}

\begin{enumerate}[resume*]
\item $\forall a\in\RR, a+(-a)=0$
\item $\forall a\in\RR, (-a)+a=0$
\item $\forall a\in\RR, a\neq0\implies a\cdot a^{-1} = 1$
\item $\forall a\in\RR, a\neq0\implies a^{-1}\cdot a = 1$
\item $-0=0$
\item $1^{-1}=1$
\end{enumerate}

\M We can prove the following results, but take them as axioms.
\begin{enumerate}[resume*]
\item $\forall a\in\RR, -(-a)=a$
\item $\forall a,b\in\RR, a-b = a+(-b)$
\item $\forall a,b\in\RR, b\neq0\implies a/b=a\cdot(b^{-1})$
\item $\forall a,b\in\RR, a\neq0\land b\neq0\implies (a\cdot b)^{-1}=(a^{-1})\cdot(b^{-1})$
\item $\forall a\in\RR, -a = (-1)\cdot a$
\item $\forall a\in\RR, a\neq=0\implies (a^{-1})^{-1}=a$
\item $\forall a,b\in\RR, (-a)\cdot(-b)=a\cdot b$
\item $\forall a,b\in\RR, (-a)\cdot b=-(a\cdot b)$
\item $\forall a,b\in\RR, a\cdot(-b)=-(a\cdot b)$
\item $\forall a,b\in\RR, b\neq0\implies (-a)/b=-(a/b)$
\item $\forall a,b\in\RR, b\neq0\implies a/(-b)=-(a/b)$
\end{enumerate}

\N{Cancellation Laws}
\begin{enumerate}[resume*]
\item $\forall a,b,c\in\RR, a+b=a+c\implies b=c$
\item $\forall a,b,c\in\RR, b+a=c+a\implies b=c$
\item $\forall a,b,c\in\RR, a\neq0\land a\cdot b=a\cdot c\implies b=c$
\item $\forall a,b,c\in\RR, a\neq0\land b\cdot a=c\cdot a\implies b=c$
\end{enumerate}

\N{Other identities}
These may be derived as theorems, but we can take them as axioms.
\begin{enumerate}[resume*]
\item $\forall a,b\in\RR, a^{2} - b^{2} = (a-b)(a+b)$
\item $\forall a,b\in\RR, a^{2} + 2ab + b^{2} = (a+b)^{2}$
\item $\forall a,b\in\RR, a^{2} - 2ab + b^{2} = (a-b)^{2}$
\item $\forall a,b,x\in\RR, x^{2} + (a+b)\cdot x + a\cdot b = (x+a)\cdot(x+b)$
\item $\forall a,b,c,d\in\RR, (a+b)(c+d) = ac+ad+bc+bd$
\item $\forall a,b,c,d\in\RR, b\neq0\land d\neq0\implies (a/b)\cdot(c/d) = (a\cdot c)/(b\cdot d)$
\item $\forall a,b,c,d\in\RR, b\neq0\land d\neq0\implies (a/b) + (c/d) = (a\cdot d + b\cdot c)/(b\cdot d)$
\item $\forall a,b,c,d\in\RR, b\neq0\land d\neq0\implies (a/b) - (c/d) = (a\cdot d - b\cdot c)/(b\cdot d)$
\end{enumerate}

\section{Order Laws}

\N{Trichotomy law} For any $a,b\in\RR$ exactly one of the following is
true:
\begin{equation}
a < b,\quad\mbox{or}\quad a=b,\quad\mbox{or}\quad a>b.
\end{equation}
We call $a$ \define{Positive} if $a>0$, and \define{Negative} if $a<0$.

\N{Sign Laws} We can derive the following from just $a<b\implies a+c<b+c$ and
$0<a\land 0<b\implies 0<a\cdot b$ (the axioms for an ordered field).
\begin{enumerate}[resume*]
\item $\forall a,b\in\RR, a>0\land b>0\implies ab>0\land a/b>0$
\item $\forall a,b\in\RR, a<0\land b>0\implies ab<0\land a/b<0$
\item $\forall a,b\in\RR, a>0\land b<0\implies ab<0\land a/b<0$
\item $\forall a,b\in\RR, a<0\land b<0\implies ab>0\land a/b>0$
\item $\forall a,b\in\RR, a>0\land b>0\implies a+b>0$
\item $\forall a,b\in\RR, a<0\land b<0\implies a+b<0$
\item $\forall a\in\RR, a>0\iff -a<0$
\item $\forall a\in\RR, a>0\iff a^{-1}>0$
\item $\forall a,b\in\RR, ab>0\implies (a>0\land b>0)\lor(a<0\land b<0)$
\item $\forall a,b\in\RR, ab<0\implies (a>0\land b<0)\lor(a<0\land b>0)$
\item $\forall a,b\in\RR, a/b>0\implies (a>0\land b>0)\lor(a<0\land b<0)$
\item $\forall a,b\in\RR, a/b<0\implies (a>0\land b<0)\lor(a<0\land b>0)$
\end{enumerate}

\M
We have as an immediate consequence the following result, which we take axiomatically
\begin{enumerate}[resume*]
\item $\forall a\in\RR, a^{2}\geq0$
\item $\forall a\in\RR, a^{2}>0\iff a\neq0$
\end{enumerate}

\N{Transitivity}
\begin{enumerate}[resume*]
\item $\forall a,b,c\in\RR,a<b\land b<c\implies a<c$
\end{enumerate}

\N{Addition of inequalities}
\begin{enumerate}[resume*]
\item $\forall a,b,c,d\in\RR, a<b\land c<d\implies a+c<b+d$
\item $\forall a,b,c,d\in\RR, a\leq b\land c\leq d\implies a+c\leq b+d$
\item $\forall a,b,c,d\in\RR, a<b\land c\leq d\implies a+c< b+d$
\item $\forall a,b,c\in\RR, a<b\implies a-c < b-c$
\item $\forall a,b\in\RR, a<b\implies -a > -b$
\item $\forall a,b,c\in\RR, b<c\implies a-b > a-c$
\end{enumerate}

\N{Multiplication of Inequalities}
\begin{enumerate}[resume*]
\item $\forall a,b,c,d\in\RR, a<b\land c<d\implies ac<bd$
\item $\forall a,b,c\in\RR, a<b\land c>0\implies a/c<b/c$
\item $\forall a,b,c,d\in\RR, 0<a<b\land 0<c<d\implies 0<ac<bd$
\item $\forall a,b,c\in\RR, a<b\land c<0\implies ac>bc$
\item $\forall a,b,c\in\RR, a<b\land c<0\implies a/c>b/c$
\item $\forall a,b\in\RR, 0<a\land a<b\implies a^{-1} > b^{-1}$
\end{enumerate}

\N{Arcimedean Property} This may be stated in various forms.
\begin{enumerate}[resume*]
\item $\forall a\in\RR,\exists x,y\in\QQ, x < a < y$
\item $\forall a\in\RR, a>0\implies \exists n\in\NN, a < n$
\item $\forall a,b\in\RR, a>0\land a < b\implies \exists n\in\NN, b < na$
\end{enumerate}

\section{Definitions}

\M There are a few notions worth defining, like the absolute value and
   [rational] powers.

\subsection{Absolute Value}

\begin{definition}
For any $x\in\RR$, we define the \define{Absolute Value} to be
the number $|x|\in\RR$ by
\begin{equation}
  |x| = \begin{cases}
     x & \mbox{if } x > 0,\\
     0 & \mbox{if } x = 0,\\
    -x & \mbox{if } x < 0.
  \end{cases}
\end{equation}
\end{definition}

\M Some results
\begin{enumerate}[resume*]
\item $\forall a,b\in\RR, a>0\implies (|x|<a \iff -a<x<a)$
\item $\forall a,b\in\RR, a>0\implies (|x|\leq a \iff -a\leq x\leq a)$
\item $\forall a\in\RR, |a|=|-a|$
\item $\forall a\in\RR, -|a| \leq a \leq |a|$
\item $\forall a,b\in\RR, |ab|=|a|\cdot|b|$
\item $\forall a,b\in\RR, b\neq0\implies |a/b| = |a|/|b|$
\end{enumerate}

\subsection{Powers}

\begin{definition}
Let $a\in\RR$ and $n\in\NN_{0}$, then the \define{Power} is defined by
the rules
\begin{subequations}
\begin{align}
a^{0} &= 1\\
a^{n+1} &= a^{n}\cdot a.
\end{align}
\end{subequations}
Further, if $a\neq0$ and $n\in\NN$ is nonzero, then we extend our
definition to the negative integers by
\begin{equation}
a^{-n} = \frac{1}{a^{n}}.
\end{equation}
\end{definition}

\begin{definition}
Let $a\in\RR$ and $n\in\NN$. Assume $a>0$. We define the fractional
power by
\begin{equation}
\exists!b\in\RR,b=a^{1/n}\land b^{n}=a.
\end{equation}
Now, if $a\geq0$ and $m\in\ZZ$ arbitrary and $n\in\NN$, we can define the
rational power of $a$ by
\begin{equation}
a^{m/n} = \begin{cases}
     (a^{1/n})^{m} & \mbox{if } a > 0\\
               0 & \mbox{if } a=0 \mbox{ and } m>0\\
\mbox{undefined} & \mbox{if } a=0\mbox{ and } m < 0.
\end{cases}
\end{equation}
\end{definition}

\begin{remark}
The question of $0^{0}$ is a contentious issue. We are inclined to agree
with Knuth (\arXiv{math/9205211}) that we should take $0^{0}=1$ and distinguish this
from the limits to these values. After all, $0^{0}$ permits the Binomial
theorem to make sense in more general settings, and the Binomial theorem
is too important to give up.
\end{remark}

\N{Monotonicity of Powers}
\begin{enumerate}[resume*]
\item $\forall x,y\in\RR,r\in\QQ, x\geq0\land y\geq0\land r>0\implies(x<y\iff x^{r}<y^{r})$
\item $\forall x,y\in\RR,r\in\QQ, x>0\land y>0\land r<0\implies(x<y\iff x^{r}>y^{r})$
\item $\forall a\in\RR,p,q\in\QQ, a>1\implies (p<q\iff a^{p}<a^{q})$
\item $\forall a\in\RR,p,q\in\QQ, a<1\implies (p<q\iff a^{p}>a^{q})$
\end{enumerate}

\N{Laws of Exponents} Whenever the powers involved are defined, then we
have the following identities.
\begin{enumerate}[resume*]
\item $\forall a\in\RR,\forall r,s\in\QQ,a^{r}a^{s}=a^{r+s}$
\item $\forall a\in\RR,\forall r,s\in\QQ,(a^{r})^{s}=a^{(rs)}$
\item $\forall a,b\in\RR,\forall r\in\QQ,(ab)^{r}=a^{s}b^{r}$
\item $\forall a\in\RR,\forall r\in\QQ, a^{-r} = 1/a^{r}$
\end{enumerate}

\section{Axiomatic Definition of Reals}

\subsection{Field Axioms}

\begin{axiom}
$\NN\subset\ZZ\subset\QQ\subset\RR$.
\end{axiom}

\begin{axiom}[Associativity of addition]\label{axiom:elementary-algebra:add-associativity}
For all $x$, $y$, $z\in\RR$, we have $x + (y + z) = (x + y) + z$.
\end{axiom}

\begin{axiom}[Commutativity of addition]\label{axiom:elementary-algebra:add-commutativity}
For all $x$, $y\in\RR$, we have $x + y = y + x$.
\end{axiom}

\begin{axiom}[Existence of $0$]\label{axiom:elementary-algebra:existence-of-0}
There exists a number $0\in\QQ$ such that for any $x\in\RR$ we have $x+0=x$.
\end{axiom}

\begin{proposition}\label{prop:elementary-algebra:additive-unit-identity}
Let $x\in\RR$. Then $0 + x = x$ and $x + 0 = x$.
\end{proposition}

\begin{proof}
We have $x + 0 = x$ by Axiom~\ref{axiom:elementary-algebra:existence-of-0}.
By direct calculation:
\begin{calculation}
x
\step{from Axiom~\ref{axiom:elementary-algebra:existence-of-0}}
x + 0
\step{from Axiom~\ref{axiom:elementary-algebra:add-commutativity}}
0 + x.\qedhere
\end{calculation}
\end{proof}

\begin{axiom}[Existence of additive inverse]
For all $x\in\RR$ there exists at least one $y\in\RR$ such that $x + y = 0$.
\end{axiom}

\begin{theorem}[Uniqueness of additive inverse]
Let $x\in\RR$. For any $y$, $y'\in\RR$ such that $x + y = 0$ and $x + y' = 0$,
we have $y = y'$. 
\end{theorem}

\begin{proof}
We have
\begin{calculation}
  y
\step{by $0$ being additive identity from Proposition~\ref{prop:elementary-algebra:additive-unit-identity}}
y + 0
\step{by hypothesis $0 = x + y'$}
y + (x + y')
\step{by associativity of addition from Axiom~\ref{axiom:elementary-algebra:add-associativity}}
(y + x) + y'
\step{by commutativity of addition from Axiom~\ref{axiom:elementary-algebra:add-commutativity}}
(x + y) + y'
\step{from hypothesis}
0 + y'
\step{by $0$ being additive identity from Proposition~\ref{prop:elementary-algebra:additive-unit-identity}}
y'.\qedhere
\end{calculation}
\end{proof}

\begin{remark}
Since the additive inverse is unique, we write $-x$ for the real number
such that $x + (-x) = 0$. We write $-x$ in Lisp as \lstinline[language=lisp]{(- x)}.
\end{remark}

\begin{corollary}\label{cor:elementary-algebra:add-inverse}
For any $x\in\RR$, we have $x + (-x) = 0$ and $(-x) + x = 0$.
\end{corollary}

\begin{axiom}[Associativity of multiplication]
For all $x$, $y$, $z\in\RR$, we have $x \cdot (y \cdot z) = (x \cdot y) \cdot z$.
\end{axiom}

\begin{axiom}[Commutativity of multiplication]\label{axiom:elementary-algebra:times-commutativity}
For all $x$, $y\in\RR$, we have $x \cdot y = y \cdot x$.
\end{axiom}

\begin{axiom}\label{axiom:elementary-algebra:times-distributes-over-add}
For all $x$, $y$, $z\in\RR$, we have $x\cdot(y + z) = x\cdot y + x\cdot z$.
\end{axiom}

\begin{theorem}\label{thm:elementary-algebra:times-distributes-over-add}
For all $x$, $y$, $z\in\RR$, we have $x\cdot(y + z) = x\cdot y + x\cdot z$
and $(x + y)\cdot z = x\cdot z + y\cdot z$.
\end{theorem}

\begin{proof}
We have $x\cdot(y + z) = x\cdot y + x\cdot z$ from Axiom~\ref{axiom:elementary-algebra:times-distributes-over-add}.
By direct calculation
\begin{calculation}
(x + y)\cdot z
\step{commutativity of multiplication from Axiom~\ref{axiom:elementary-algebra:times-commutativity}}
z\cdot(x + y)
\step{distributivity from Axiom~\ref{axiom:elementary-algebra:times-distributes-over-add}}
z\cdot x + z\cdot y
\step{commutativity of multiplication from Axiom~\ref{axiom:elementary-algebra:times-commutativity}}
x\cdot z + y\cdot z.\qedhere
\end{calculation}
\end{proof}

\begin{proposition}\label{prop:elementary-algebra:sub-from-both-sides}
Let $x$, $y$, $z\in\RR$. If $x + y = z$, then $x = z - y$.
\end{proposition}

\begin{axiom}[Existence of $1$]\label{axiom:elementary-algebra:times-1}
There exists a number $1\in\QQ$ such that for any $x\in\RR$ we have $x\cdot1=x$.
\end{axiom}

\begin{proposition}\label{prop:elementary-algebra:add-unit}
For all $x$, $y\in\RR$, if $x + y = x$ or $y + x = x$, then $y = 0$.
\end{proposition}

\begin{theorem}\label{thm:elementary-algebra:0-times-anything-is-0}
For any $x\in\RR$, we have $0\cdot x=0$.
\end{theorem}
\begin{proof}
By direct calculation, we find
\begin{calculation}
  x
  \step{by $1$ being multiplicative identity element}
  1\cdot x
  \step{using distributivity and $0$ being additive identity element}
  (0 + 1)\cdot x
  \step{distributivity}
  0\cdot x + 1\cdot x
  \step{since $1\cdot x=x$}
  0\cdot x + x.
\end{calculation}
We have $x = 0\cdot x + x$ imply $0\cdot x = 0$ by Proposition~\ref{prop:elementary-algebra:add-unit}.
\end{proof}

\begin{theorem}\label{thm:elementary-algebra:times-neg-1-is-add-inverse}
For any $x\in\RR$, we have $(-1)\cdot x = -x$.
\end{theorem}

\begin{proof}
We will prove $x + (-1)\cdot x = 0$, which implies $(-1)\cdot x = -x$.
By direct calculation,
\begin{calculation}
0
\step{using Theorem~\ref{thm:elementary-algebra:0-times-anything-is-0}}
0\cdot x
\step{since $0 = 1 - 1$}
(1 - 1)\cdot x
\step{distributivity}
1\cdot x + (-1)\cdot x
\step{since $1\cdot x = x$}
x + (-1)\cdot x.\qedhere
\end{calculation}
\end{proof}

\begin{proposition}
$(-1)^{2}=1$.
\end{proposition}

\begin{proof}
We find
\begin{calculation}
(-1)^{2} + (-1)
\step{distributivity}
(-1)\cdot((-1) + 1)
\step{since $(-1)+1=0$}
(-1)\cdot0
\step{since $x\cdot0=0$}
0.
\end{calculation}
It follows that $(-1)^{2}$ has the same additive invese as $1$, which
implies the result.
\end{proof}

\begin{axiom}\label{axiom:elementary-algebra:0-neq-1}
$0\neq1$.
\end{axiom}

\begin{remark}
This seems like a silly axiom, but without it we could end up with
models with the property ``Every real number is zero''. We also do not
have sufficient axioms to prove $0\neq1$.
\end{remark}

\begin{axiom}
For all $x\in\RR$, if $x\neq0$, then there exists at least one $y\in\RR$
such that $x\cdot y=1$.
\end{axiom}

\begin{theorem}
For all $x\in\RR$, if $x\neq0$, then there exists exactly one $y\in\RR$
such that $x\cdot y=1$.
\end{theorem}

\begin{proof}
Let $y$, $y'\in\RR$ be such that $x\cdot y=1$ and $x\cdot y'=1$.
Then
\begin{calculation}
  y
  \step{multiplicative unit}
  y\cdot 1
  \step{by hypothesis}
  y\cdot(x\cdot y')
  \step{associativity of multiplication}
  (y\cdot x)\cdot y'
  \step{commutativity of multiplication}
  (x\cdot y)\cdot y'
  \step{by hypothesis}
  1\cdot y'
  \step{multiplicative unit}
  y'.\qedhere
\end{calculation}
\end{proof}

\begin{remark}
We will write $x^{-1}\in\RR$ to denote the real number for which $x\cdot x^{-1}=1$.
\end{remark}

\subsection{Ordered Field Axioms}

\M
We assume there is an ordering relation $\leq$ on $\RR$. The axioms we
stipulate amount to demanding $\RR$ be totally ordered and compatibility
of $\leq$ with arithmetic operations.

\N{Notation}
For $x$, $y\in\RR$, we will write
\begin{equation}
x < y\qquad\mbox{if}\qquad x\leq y\quad\mbox{and}\quad x\neq y.
\end{equation}
We also have
\begin{equation}
y > x\quad\mbox{means}\quad x < y,
\end{equation}
and
\begin{equation}
y\geq x\quad\mbox{means}\quad x\leq y.
\end{equation}

\begin{axiom}[$\leq$ is Reflexive]\label{axiom:elementary-algebra:order-reflexivity}
For all $x\in\RR$, we have $x\leq x$
\end{axiom}

\begin{axiom}[$\leq$ is Antisymmetric]\label{axiom:elementary-algebra:order-antisymmetry}
For all $x$, $y\in\RR$, if $x\leq y$ and $y\leq x$, then $x=y$.
\end{axiom}

\begin{axiom}[$\leq$ is Transitive]\label{axiom:elementary-algebra:order-transitivity}
For all $x$, $y$, $z\in\RR$, if we have $x\leq y$ and $y\leq z$,
then $x\leq z$.
\end{axiom}

\begin{axiom}[$\leq$ is Total]\label{axiom:elementary-algebra:order-total}
For all $x$, $y\in\RR$, either $x\leq y$ or $y\leq x$.
\end{axiom}

\begin{proposition}\label{prop:elementary-algebra:order-total}
For all $x$, $y\in\RR$, either $x < y$ or $x = y$ or $x > y$.
\end{proposition}

\begin{axiom}[$\leq$ Preserved Under Addition]\label{axiom:elementary-algebra:add-preserves-order}
For all $x$, $y$, $z\in\RR$, if $x\leq y$, then $x + z\leq y + z$.
\end{axiom}

\begin{proposition}
For all $x$, $y$, $z\in\RR$, if $x < y$, then $x + z < y + z$.
\end{proposition}

\begin{theorem}
$-1 < 0$.
\end{theorem}

\begin{proof}
Add $1$ to both sides yields $0\leq 1$. We have $0\neq1$ by Axiom~\ref{axiom:elementary-algebra:0-neq-1}.
\end{proof}

\begin{axiom}[$\leq$ Preserved Under Multiplication]\label{axiom:elementary-algebra:times-preserves-order}
For all $x$, $y\in\RR$, if $0\leq x$ and $0\leq y$, then $0 \leq x\cdot y$.
\end{axiom}

\begin{definition}
Let $x\in\RR$.
\begin{enumerate}
\item We call $x$ \define{Positive} if $x > 0$.
\item We call $x$ \define{Negative} if $x < 0$.
\item We call $x$ \define{Non-negative} if $x\geq 0$.
\item We call $x$ \define{Non-positive} if $x\leq 0$.
\end{enumerate}
\end{definition}

\subsection{Exponentiation}

\begin{definition}
Let $x\in\RR$, let $n\in\NN_{0}$.
We inductively define the $n^{\text{th}}$ power of $x$ by:
\begin{enumerate}
\item $x^{0} = 1$
\item $x^{n + 1} = x^{n}\cdot x$.
\end{enumerate}
\end{definition}

\begin{remark}
This means $0^{0}=1$, when it should be undefined. We make this decision
so we can obtain the binomial theorem.
\end{remark}

\begin{remark}
The Lisp function for $x^{n}$ is \lstinline[language=lisp]{(expt} $x$ $n$\lstinline[language=lisp]{)}.
\end{remark}

\begin{proposition}
Let $x\in\RR$. Then $x^{1} = x$.
\end{proposition}

\begin{definition}
Let $x\in\RR$ be nonzero, let $n\in\NN$.
We extend the $n^{\text{th}}$ power of $x$ to negative values of $n$ by
\begin{equation}
x^{-n} = (x^{n})^{-1}.
\end{equation}
That is, $x^{-n}$ is the multiplicative inverse of $x^{n}$.
\end{definition}

\begin{remark}
This justifies the choice of notation that $x^{-1}$ is the
multiplicative inverse of $x$, since we would have $x^{-1} = (x^{1})^{-1}$
--- or to be explicitly clear in Lisp notation, 
\lstinline[language=lisp]{(expt x -1)} is equal to
\lstinline[language=lisp]{(/ (expt x 1))}. But since $x^{1}=x$, we have
\lstinline[language=lisp]{(expt x -1)} equal to \lstinline[language=lisp]{(/ x)}.
This identification is made readily by our choice of notation.
\end{remark}

\begin{proposition}
For any $x\in\RR$, $m$, $n\in\NN_{0}$, we have $(x^{m})\cdot(x^{n})=x^{m+n}$.
\end{proposition}

\begin{proof}
By induction on $n$.

Base case ($n=0$): by direct calculation
\begin{calculation}
  (x^{m})\cdot(x^{0})
  \step{since $x^{0}=1$}
  (x^{m})\cdot1
  \step{since $1$ is unit of multiplication}
  x^{m}
  \step{since $m = m+0$}
  x^{m+0}
  \step{since $n=0$}
  x^{m+n}.
\end{calculation}

Inductive hypothesis: assume $(x^{m})\cdot(x^{n})=x^{m + n}$.

Inductive case: we see
\begin{calculation}
  (x^{m})\cdot(x^{n+1})
  \step{by definition}
  (x^{m})\cdot(x^{n}\cdot x)
  \step{associativity of multiplication}
  \bigl((x^{m})\cdot(x^{n})\bigr)\cdot x
  \step{by inductive hypothesis}
  x^{m + n} \cdot x
  \step{by definition}
  x^{(m + n) + 1}
  \step{by associativity of addition}
  x^{m + n + 1}.\qedhere
\end{calculation}
\end{proof}

\begin{corollary}
For any nonzero $x\in\RR$, and for any $m$, $n\in\ZZ$,
we have $(x^{m})\cdot(x^{n})=x^{m+n}$.
\end{corollary}

\begin{proposition}
For any $x\in\RR$, $m$, $n\in\NN_{0}$, we have $(x^{m})^{n}=x^{mn}$.
\end{proposition}

\begin{proof}
By induction on $n$.

Base case ($n=0$): $(x^{m})^{0} = 1$ by definition.

Inductive hypothesis: assume $(x^{m})^{n}=x^{mn}$.

Inductive case: we see
\begin{calculation}
  (x^{m})^{n+1}
  \step{by definition}
  \bigl((x^{m})^{n}\bigr)\cdot(x^{m})
  \step{by inductive hypothesis}
  x^{mn}\cdot x^{m}
  \step{using $x^{a}x^{b}=x^{a+b}$}
  x^{mn + m}
  \step{distributivity gives $m\cdot(n + 1) = mn + m$}
  x^{m\cdot(n + 1)}.\qedhere
\end{calculation}
\end{proof}

\begin{lemma}
For any nonzero $x\in\RR$, and for any $n\in\NN$, we have $x^{-n}=(x^{n})^{-1}=(x^{-1})^{n}$.
\end{lemma}

\begin{proof}
Since $x^{-n} = (x^{n})^{-1}$ by definition of exponentiation to a
negative power, we are left to prove $x^{-n} = (x^{-1})^{n}$.

By induction on $n$. The base case ($n=1$) is $x^{-1} = (x^{1})^{-1}$
which is true, and $(x^{-1})^{1} = (x^{-1})$.

Inductive hypothesis: assume for arbitrary $n$ that $x^{-n}=(x^{n})^{-1}=(x^{-1})^{n}$.

Inductive case: we have $x^{-(n+1)} = (x^{n+1})^{-1}$ by
definition.
From $x^{n+1} = x^{n}x^{1}$ we have
$(x^{n+1})^{-1} = (x^{n}x^{1})^{-1} = (x^{n})^{-1}(x^{1})^{-1} = x^{-n} x^{-1}$,
Using the inductive hypothesis $x^{-n} = (x^{-1})^{n}$ we arrive at $(x^{n+1})^{-1}=(x^{-1})^{n}x^{-1}=(x^{-1})^{n+1}$,
as desired.
\end{proof}

\begin{corollary}\label{cor:elementary-algebra:expt-of-expt-is-expt-raised-to-product}
For any nonzero $x\in\RR$, and for any $m$, $n\in\ZZ$,
we have $(x^{m})^{n}=x^{mn}$.
\end{corollary}

\begin{proof}
Since $n\geq 0$ or $n < 0$, we prove it by cases.

Assume $n\geq 0$. Either $m\geq0$ or $m < 0$. For $m\geq 0$,
the result follows immediately. For $m < 0$, write $m = -k$, then
$x^{m} = x^{-k} = (x^{-1})^{k}$. But $x^{-1}$ is a real number and $k\geq0$.
So $((x^{-1})^{k})^{n}=(x^{-1})^{kn}$. And by definition $(x^{-1})^{kn}=x^{-kn}=x^{mn}$.

For $n < 0$, let us write $n=-q$. Then $(x^{m})^{n} = (x^{m})^{-q} = [(x^{m})^{q}]^{-1}=(x^{mq})^{-1}=x^{-mq}=x^{-mn}$.
\end{proof}

\begin{corollary}
For any nonzero $x\in\RR$ and for any $n\in\ZZ$, we have $x^{2n} = (x^{2})^{n}$.
\end{corollary}

\begin{proof}
This follows from Corollary~\ref{cor:elementary-algebra:expt-of-expt-is-expt-raised-to-product}
with $m=2$.
\end{proof}

\begin{remark}
This will be useful when computing $x^{n}$, since either $n=2k$ or
$n=2k+1$. In the former case, we recursively compute $(x^{2})^{k}$, and
the latter case we computer $x^{n} = x\cdot x^{2k} = x\cdot (x^{2})^{k}$.
\end{remark}

\begin{proposition}
For any $x\in\RR$, we have $0\leq x^{2}$.
\end{proposition}

\begin{proof}
From Proposition~\ref{prop:elementary-algebra:order-total},
we have $x < 0$ or $x = 0$ or $x > 0$. We will work in these three
cases.

If $x < 0$, then write $x = -y$ for $y\in\RR$ with $y > 0$. Then $x^{2} = (-1)^{2}y^{2}$.
Since $(-1)^{2} = 1$, this implies $x^{2} = y^{2}$ and $y^{2}\geq 0$ by Axiom~\ref{axiom:elementary-algebra:times-preserves-order}.

If $x = 0$, then $x^{2}=0$. Hence the result.

If $x > 0$, then $x\geq 0$, and the result follows from Axiom~\ref{axiom:elementary-algebra:times-preserves-order}.
\end{proof}

% \label{axiom:elementary-algebra:}

\section{Binomial Theorem}

\begin{definition}
Let $n\in\NN_{0}$. We define the \define{Factorial} of $n$ to be
inductively defined by,
\begin{equation}
  n! = \begin{cases}1 & \mbox{if }n=0\\
    n\cdot((n-1)!) & \mbox{otherwise}
  \end{cases}
\end{equation}
\end{definition}

\begin{definition}
Let $m$, $n\in\NN_{0}$. We define the \define{Binomial Coefficient} for
$0\leq m\leq n$ as:
\begin{subequations}
\begin{equation}
\binom{n}{m} = \frac{n!}{m!(n-m)!}.
\end{equation}
If $m > n$, then we define
\begin{equation}
\binom{n}{m} = 0.
\end{equation}
\end{subequations}
\end{definition}

\begin{remark}
We can weaken this definition a little, allowing us to define for any
$x\in\RR$ and $k\in\NN_{0}$ the \define{Generalized Binomial Coefficient}
\begin{equation}
\binom{x}{k} = \frac{x(x-1)(x-2)(\cdots)(x-(k-1))}{k!}.
\end{equation}
\end{remark}

\begin{proposition}\label{prop:elementary-algebra:binomial-coef:complement-bottom}
  For $k$, $n\in\NN_{0}$, we have
  \begin{equation}
\binom{n}{k} = \binom{n}{n-k}.
  \end{equation}
\end{proposition}

\begin{theorem}[Pascal's identity]\label{thm:elementary-algebra:pascal-identity}
  For any $k$, $n\in\NN$, we have
  \begin{equation}
\binom{n - 1}{k} + \binom{n - 1}{k-1} = \binom{n}{k}.
  \end{equation}
\end{theorem}

\begin{proof}
By direct calculation, we have:
\begin{calculation}
\binom{n-1}{k} + \binom{n-1}{k-1}
\step{unfold definition of binomial coefficient}
\frac{(n-1)!}{k!(n - 1 - k)!} + \frac{(n - 1)!}{(k - 1)! (n - k)!}
\step{distributivity}
(n - 1)!\left[\frac{1}{k!(n - 1 - k)!} + \frac{1}{(k - 1)! (n - k)!}\right]
\step{multiply by $1=(n-k)/(n-k)$ and $1=k/k$}
(n - 1)!\left[\frac{1}{k!(n - 1 - k)!}\frac{n-k}{n-k} + \frac{1}{(k - 1)! (n - k)!}\frac{k}{k}\right]
\step{folding in the definition of factorial}
(n - 1)!\left[\frac{n - k}{k!(n - k)!} + \frac{k}{k! (n - k)!}\right]
\step{algebra}
(n - 1)!\left[\frac{n}{k!(n - k)!}\right]
\step{folding in the definition of factorial}
\frac{n!}{k!(n - k)!}
\step{folding in definition of binomial coefficient}
\binom{n}{k}.\qedhere
\end{calculation}
\end{proof}

\begin{lemma}\label{lemma:elementary-algebra:binomial-theorem-helper}
For any $n\in\NN_{0}$, $y\in\RR$, we have
\begin{equation}
(1 + y)^{n} = \sum^{n}_{k=0}\binom{n}{k}y^{n-k}.
\end{equation}
\end{lemma}
\begin{proof}
By induction on $n\in\NN_{0}$.

Base case ($n = 0$): we see $(1 + y)^{0} = 1$ and $\sum^{0}_{k=0}\binom{0}{0}y^{0}=1$,
which proves the claim.

Inductive hypothesis, we assume
\begin{equation}%\label{eq:lemma:elementary:binomial-theorem-helper:inductive-hypothesis}
(1 + y)^{n} = \sum^{n}_{k=0}\binom{n}{k}y^{n-k}.
\end{equation}
We observe, reindexing this sum to work with ascending powers of $y$,
then applying the fact, from Proposition~\ref{prop:elementary-algebra:binomial-coef:complement-bottom},
that
\[\binom{n}{k} = \binom{n}{n-k},\]
we find
\begin{equation}\label{eq:lemma:elementary:binomial-theorem-helper:inductive-hypothesis}
(1 + y)^{n} = \sum^{n}_{k=0}\binom{n}{k}y^{k}.
\end{equation}
Now we want to prove the rule holds for $n+1$. We see
\begin{calculation}
(1 + y)^{n+1}
\step{algebra}
(1 + y)^{n}(1 + y)
\step{distributivity}
(1 + y)^{n} + y(1 + y^{n})
\step{using inductive hypothesis Eq~\eqref{eq:lemma:elementary:binomial-theorem-helper:inductive-hypothesis}}
\left(\sum^{n}_{k=0}\binom{n}{k}y^{k}\right) + y\left(\sum^{n}_{k=0}\binom{n}{k}y^{k}\right)
\step{distributivity in second term}
\left(\sum^{n}_{k=0}\binom{n}{k}y^{k}\right) + \left(\sum^{n}_{k=0}\binom{n}{k}y^{k+1}\right)
\step{breaking out the leading term in first sum}
\left(1 + \sum^{n}_{k=1}\binom{n}{k}y^{k}\right) + \left(\sum^{n}_{k=0}\binom{n}{k}y^{k+1}\right)
\step{breaking out the last term in the second sum}
\left(1 + \sum^{n}_{k=1}\binom{n}{k}y^{k}\right) + \left(y^{n+1} + \sum^{n-1}_{k=0}\binom{n}{k}y^{k+1}\right)
\step{reindexing second term}
\left(1 + \sum^{n}_{k=1}\binom{n}{k}y^{k}\right) + \left(y^{n+1} + \sum^{n}_{k=1}\binom{n}{k-1}y^{k}\right)
\step{associativity of addition, combine sums}
1 + \left(\sum^{n}_{k=1}\left[\binom{n}{k}+\binom{n}{k-1}\right]y^{k}\right)
+ y^{n + 1}
\step{using Pascal's identity from Theorem~\ref{thm:elementary-algebra:pascal-identity}}
1 + \left(\sum^{n}_{k=1}\binom{n+1}{k}y^{k}\right)
+ y^{n + 1}
\step{absorbing the first and last terms into the sum}
\sum^{n+1}_{k=0}\binom{n+1}{k}y^{k}.\qedhere
\end{calculation}
\end{proof}

\begin{theorem}[Binomial]
For any $n\in\NN_{0}$, $x$, $y\in\RR$, we have
\begin{equation}
(x + y)^{n} = \sum^{n}_{k=0}\binom{n}{k}x^{k}y^{n-k}.
\end{equation}
\end{theorem}

\begin{proof}
The proof is per cases on whether $x=0$ or $x\neq0$.

\textbf{Case 1:} If $x=0$, then the proof is trivial. Then the right-hand side of the
claim has its sum keep only its first term, giving us
\begin{equation}
(0 + y)^{n} = \binom{n}{0}y^{n}.
\end{equation}
This is trivially true.

\textbf{Case 2:} We assume $x\neq0$. Then
\begin{calculation}
  (x + y)^{n}
\step{factor out $x$}
  x^{n}\left(1 + \frac{y}{x}\right)^{n}
\step{using Lemma~\ref{lemma:elementary-algebra:binomial-theorem-helper}}
x^{n}\sum^{n}_{k=0}\binom{n}{k}\left(\frac{y}{x}\right)^{n-k}
\step{algebra}
x^{n}\sum^{n}_{k=0}\binom{n}{k}x^{-(n-k)}y^{n-k}
\step{distributivity}
\sum^{n}_{k=0}\binom{n}{k}x^{n}x^{-(n-k)}y^{n-k}
\step{algebra}
\sum^{n}_{k=0}\binom{n}{k}x^{k}y^{n-k}.\qedhere
\end{calculation}
\end{proof}

\begin{remark}
The Binomial series generalizes the binomial theorem, by replacing $n$
with $\alpha\in\RR$, then using the series
\begin{equation}
(1 + x)^{\alpha} = \sum^{\infty}_{k = 0}\binom{\alpha}{k}x^{k}
= 1 + \alpha x + \frac{\alpha(\alpha-1)}{2!}x^{2} + \frac{\alpha(\alpha-1)(\alpha-2)}{3!}x^{3}+\cdots.
\end{equation}
This uses the generalized binomial coefficients, and reduces to the
familiar Binomial expansion for $\alpha\in\NN_{0}$. We can observe that
this is just the Taylor series expansion in $x$ about $0$.
\end{remark}

\section{Series and Sums}

\M
This is a sticky issue, because summation methods can assign numbers and
closed-form expressions to divergent series. Hardy, in his book
\textit{Divergent Series}, talks about a
``Pickwickian summation scheme''; the desired qualities for any
summation scheme are twofold:
\begin{enumerate}
\item linear $c\sum_{n}a_{n}=\sum_{n}(ca_{n})$ and $(\sum_{n}a_{n})+(\sum_{n}b_{n})=\sum_{n}(a_{n}+b_{n})$
\item we can pull out the first term: $\sum_{n=1}a_{n} = a_{1} + \sum_{n=2}a_{n}$.
\end{enumerate}
More explicitly, if $P(-)$ is the Pickwickian summation scheme,
\begin{enumerate}
\item If $P(\sum a_{n})=s$, then $P(\sum c\cdot a_{n})=c\cdot s$;
\item If $P(\sum a_{n})=s$ and $P(\sum b_{n})=t$, then $P(\sum a_{n} + b_{n})=s+t$;
\item If $P(\sum_{n=1} a_{n})=s$, then $P(\sum_{n=2} a_{n})=s-a_{1}$.
\end{enumerate}

\M
Ferraro argues that Euler used two methods for determining sums: the
binomial theorem, and something Ferraro calls ``the method of
indeterminate coefficients''. What Ferraro means by this is: consider a
power series expansion for the fraction
\begin{equation}
f(x) = \frac{c}{b + x}.
\end{equation}
We assume there exists a series $\sum_{n=0}a_{n}x^{n}$ such that
\begin{subequations}
\begin{align}
c &= (b + x)\sum^{\infty}_{n=0}a_{n}x^{n}\\
&= (b + x)(a_{0} + a_{1}x + a_{2}x^{2} + \cdots)\\
&= ba_{0} + ba_{1}x + ba_{2}x^{2} + \cdots\nonumber\\
&\phantom{= ba_{0}} + a_{0}x + a_{1}x^{2} + \cdots\\
&= ba_{0} + (ba_{1} + a_{0})x + (ba_{2} + a_{1})x^{2} + \cdots.
\end{align}
\end{subequations}
Then we match coefficients to find
\begin{subequations}
\begin{align}
c &= ba_{0}\\
0 &= ba_{1} + a_{0}\\
0 &= ba_{2} + a_{1}
\end{align}
\end{subequations}
and so on. This determines the unknown coefficients $a_{0}=c/b$, and
$a_{n+1}=-a_{n}/b$ for each $n\in\NN_{0}$.

% http://fredrickey.info/hm/Euler-Introductio.pdf

\begin{theorem}[Geometric series]
Let $a\in\RR$, $N\in\NN$. Then
\begin{equation}
\sum^{N}_{n=0}a^{n} = \frac{1 - a^{N+1}}{1 - a}.
\end{equation}
\end{theorem}

\begin{proof}
  We see
  \begin{equation}
(1 - a)(1 + a + a^{2} + \dots + a^{N}) = 1 - a^{N+1}.
  \end{equation}
  Dividing both sides by $1-a$ then produces the result.
For $N>1$, we have explicitly:
\begin{calculation}
(1 - a)(1 + a + a^{2} + \dots + a^{N-1} + a^{N})
\step{associativity of addition}
(1 - a)(1 + (a + a^{2} + \dots + a^{N-1}) + a^{N})
\step{distributivity}
1\cdot(1 + (a + a^{2} + \dots + a^{N-1}) + a^{N}) - a(1 + (a + a^{2} + \dots + a^{N-1}) + a^{N})
\step{distributivity}
(1 + (a + a^{2} + \dots + a^{N-1}) + a^{N}) -a - (a^{2} + \cdots + a^{N}) - a^{N+1}
\step{associativity, distributivity}
1 + (a + a^{2} + \dots + a^{N-1} + a^{N}) - (a + a^{2} + \cdots + a^{N}) - a^{N+1}
\step{definition of subtraction}
1 + 0 - a^{N+1}.
\end{calculation}
Dividing both sides by $1-a$ yields the results.
\end{proof}

\section{Concluding Remarks}

\M
These are just random thoughts I should organize better. It's not a
``conclusion'' \textit{per se}, just ``here's stuff I wrote that doesn't
fit in with the existing sections''.

\N{Existence of Squareroots}
We define, e.g., $x^{1/n}$ to be ``the $y\in\RR$'' such that $y^{n}=x$.
Why should we believe such a $y$ even exists? More precisely, why should
\emph{the computer} believe it? I guess we could have a definitional
axiom of the form ``$\forall n\forall x, n\in\ZZ\land x\in\RR\land x\geq0\implies\exists y,y^{n}=x$''.
Or in pidgin Lisp,

\begin{lisp-example}
(defaxiom nth-root ((n int) (x real))
  (implies (not (neg? x))
           (= (expt (expt x (/ n)) n) x)))
\end{lisp-example}

Euler's \textit{Elements of Algebra} (part I, chapter XII, ``Of square
roots and of Irrational Numbers resulting from them'') seemed to adopt
the perspective that we could, for any $x\geq1$, 
find an integer $M$ such that $M^{k}\leq x < (M+1)^{k}$. We then form
two sequences $a_{n}$, $b_{n}$ which are inductively defined by the same
recurrence relation
\begin{equation}
x_{n+1} = \frac{1}{n}\left[(n-1)x_{n} + \frac{x}{x_{n}^{k-1}}\right],
\end{equation}
which is Newton's method for the $k^{\text{th}}$ root of $x$, starting
with initial values $a_{1}=M$ and $b_{1}=M+1$. Then for every $n\in\NN$,
we have $a_{n}<a_{n+1}\leq x^{1/k}\leq b_{n+1}<b_{n}$. We can therefore
approximate $x^{1/k}$ as a rational number to arbitrary $\varepsilon>0$.
(For $0<x<1$, we pick $M$ such that $(M+1)^{-k}\leq x < M^{-k}$,
and use initial values $a_{1} = 1/(M + 1)$, $b_{1} = 1/M$.)

Since Newton's method converges quadratically for suitable initial
choices, it helps to consider $\alpha = \lfloor x\rfloor$, then the
number of bits being $\beta$, guess $a_{1}=2^{\lfloor \beta/k\rfloor}$
and analogously for $b_{1}$ using ceiling functions instead. This has
the advantage of using Common Lisp's \lstinline[language=lisp]{integer-length}
to compute the number of bits necessary to represent an integer in
twos-complement representation.

\begin{lisp-example}
(defun newton-nth-root-step (guess x n)
  (/ (+ (* (- n 1) guess)
        (/ x (expt guess (- n 1))))
     n))

(defun newton-nth-root-iter (a b x n tolerance)
  (if (<= (- b a) tolerance)
    (/ (+ a b) 2)
    (newton-nth-root-iter (newton-nth-root-step a x n)
                          (newton-nth-root-step b x n)
                          x
                          n
                          tolerance)))

;; Assumes x > 1.
(defun newton-nth-root (x n tolerance)
  (let ((initial-a (expt 2 (floor (/ (integer-length (floor x)) k))))
        (initial-b (expt 2 (ceiling (/ (integer-length (ceiling x)) k)))))
    (newton-nth-root-iter initial-a initial-b x n tolerance)))

;; Assumes x >= 0, n > 0.
(defun nth-root-for-positive (x n tolerance)
  (if (or (zero? x) (= 1 x))
    x
    (if (< 0 x 1)
       (/ (newton-nth-root (/ x) n tolerance))
       (newton-nth-root x n tolerance))))

;; The :branch argument is if we want to consider a different
;; branch than the principal branch (default value). Since `x`
;; is the same as `(* x (exp (* 2 pi #c(0 1) k)))`, taking the nth
;; root returns n possible values differing by a factor of
;;`(exp (* 2 pi #c(0 1) (/ branch n)))` where `branch` is the optional value. 
(defun nth-root-for-real ((x real) n tolerance &keyword (branch 0))
  (* (if (zero? branch)
       1
       (expt (root-of-unity n) branch))  ; = (exp (* 2 pi #c(0 1) (/ branch n)))
     (nth-root-for-positive (abs x) n tolerance)
     (if (neg? x)
       #c((cos (/ pi n)) (sin (/ pi n))) ; = (expt -1 (/ n))
       1)))
\end{lisp-example}

\begin{remark}
  Euler calls them ``determinate quantities''. Well, here's the passage
  from Chapter XII, Part I, of his \textit{Elements of Algebra}:

  \begin{quotation}
    128. There is, therefore, a sort of numbers, which
cannot be assigned by fractions, but which are nevertheless determinate quantities; as, for instance, the square
root of 12: and we call this new species of numbers,
\emph{irrational numbers}. They occur whenever we endeavour
to find the square root of a number which is not a square;
thus, 2 not being a perfect square, the square root of 2,
or the number which multiplied by itself would produce 2,
is an irrational quantity. These numbers are also called
\emph{surd quantities}, or \emph{incommensurable}.

129. These irrational quantities, though they cannot be
expressed by fractions, are nevertheless magnitudes of which
we may form an accurate idea; since, however concealed
the square root of 12, for example, may appear, we are not
ignorant that it must be a number, which, when multiplied
by itself, would exactly produce 12; and this property is
sufficient to give us an idea of the number, because it is in
our power to approximate towards its value continually.
  \end{quotation}
  Emphasis is Euler's.
\end{remark}

\N{On Completeness}
Typically there is discussion about the least-upper bound property
(``Dedekind completeness''). This is equivalent to assuming the
Archimedean property (for every positive $x\in\RR$, there exists an
$n\in\NN$ such that $1 < nx$), and that every Cauchy sequence of real numbers
converges to a real number (i.e., the reals are ``topologically complete'').

\N{Sums}
I need to insert results concerning sums before discussing the Binomial
theorem, things like reindexing results, etc.

\N{Bootstrapping Principle}
Let $P[x]$ be a predicate of real numbers $x\in\RR$.
Let $a\in\RR$.
If
\begin{enumerate}
\item $P[a]$ is true; and
\item if there exists a sequence $(x_{n})$ approaching $x$ from below, such
  that $\forall n,P[x_{n}]$, then $P[x]$ is true; and
\item if $P[x_{0}]$ is true, then there exists some $x_{1} > x_{0}$
  such that $P[x_{1}]$ is true; and
\item if $P[x_{0}]$ is true, then $P[x_{1}]$ is true for all $a<x_{1}<x_{0}$;
\end{enumerate}
then $P[x]$ is true for all $x\in[a,\infty)$.

\bigbreak
See also \arXiv{1208.0973}.

Let $a\in\RR$.
\begin{enumerate}
\item $P[a]$
\item There is a $\Delta>0$ such that $\forall x\in\RR$, $P[x]$ implies
  $\forall t\in(x-\Delta,x+\Delta)\cap[a,\infty)$, $P[t]$.
\end{enumerate}
Then $\forall x\in[a,\infty),P[x]$.