\chapter{Mathematical Results}

\begin{theorem}[Gaussian Integral]
$\displaystyle\int^{\infty}_{-\infty}\E^{-x^{2}}\,\D x = \sqrt{\pi}$.
\end{theorem}

\begin{proof}
  Let
  \begin{equation}
I = \int^{\infty}_{-\infty}\E^{-x^{2}}\,\D x.
  \end{equation}
  Then
\begin{calculation}
  I^{2}
  \step{unfold}
\int^{\infty}_{-\infty} \int^{\infty}_{-\infty}\E^{-x^{2}-y^{2}}\,\D x\,\D y
\step{change to polar coordinates}
\int^{\infty}_{0}\int^{2\pi}_{0}\E^{-r^{2}}r\,\D\theta\,\D r
\step{since integrand is constant with respect to $\theta$}
2\pi\int^{\infty}_{0}\E^{-r^{2}}r\,\D r
\step{change coordinates with $u=r^{2}$, $\D u = 2r\,\D r$}
\pi\int^{r=\infty}_{r=0}\E^{-u}\,\D u
\step{simple integration}
\left.-\pi\E^{-r^{2}}\right|^{r=\infty}_{r=0}
\step{substitution}
-\pi\E^{-\infty}+\pi\E^{-0} = \pi.
\end{calculation}
Therefore $I=\pm\sqrt{\pi}$. Since the integrand is always positive, we
conclude $I=\sqrt{\pi}$ as desired.
\end{proof}

\begin{corollary}\label{cor:math:general-gaussian-integral-in-one-dim}
Let $a,b\in\CC$. Then $\displaystyle\int^{\infty}_{-\infty}\E^{-a(x-b)^{2}}\,\D x = \sqrt{\frac{\pi}{a}}$
\end{corollary}
